bloom-filter/Spec.BloomFilter.fst
@@ -9,46 +9,103 @@ module Isize = FStar.Int32
 module I32 = FStar.Int32
 
 open Rust
+open FStar.List.Tot.Base
 
 assume type element: eqtype
 
 assume val hash: element -> u32
 
+type count = n:nat{n > 0}
+
+let contains (#a:eqtype) (l:list (a & count)) (e:a) : Tot bool =
+  existsb (fun (e', _) -> e = e') l
+
+let rec no_duplicates (#a:eqtype) (l:list (a & count)) : Tot bool (decreases l) =
+  match l with
+  | [] -> true
+  | (e, _)::tl -> not (contains tl e) && no_duplicates tl
+
+type count_list (a:eqtype) = (l:list (a & count){no_duplicates l})
+
+let same_elements (#a: eqtype) (l1 l2: count_list a) =
+  (forall (e:a). contains l1 e <==> contains l2 e)
+
+val incr_count:
+  #a:eqtype ->
+  l:count_list a ->
+  e : a{contains l e} ->
+  Tot (l':count_list a{same_elements l l'}) (decreases l)
+let rec incr_count #a l e =
+  match l with
+  | [] -> l
+  | (e', old_count)::tl ->
+    if e = e' then
+      (e', old_count + 1)::tl
+    else
+      (e', old_count)::(incr_count tl e)
+
+val element_count: #a:eqtype ->
+  l:count_list a ->
+  e: a ->
+  Tot nat (decreases l)
+let rec element_count #a l e = match l with
+  | [] -> 0
+  | (e', count)::tl ->
+    if e = e' then count else element_count tl e
+
+val decr_count:
+  #a:eqtype ->
+  l:count_list a ->
+  e : a{contains l e} ->
+  Tot (l':count_list a{
+    if element_count l e > 1 then
+      same_elements l l'
+    else begin
+      not (contains l' e) /\
+      (forall (e':a{e' <> e}). contains l e' <==> contains l' e')
+    end
+  }) (decreases l)
+let rec decr_count #a l e =
+  match l with
+  | [] -> l
+  | (e', old_count)::tl ->
+    if e = e' && old_count = 1 then
+      tl
+    else if e = e' && old_count > 1 then
+      (e', old_count - 1)::tl
+    else
+      (e', old_count)::(decr_count tl e)
+
 noeq type spec_bloom_storage_u8 = {
-   map: FStar.Map.t element nat;
-   elements: list element
+   elements: (l:(count_list element){no_duplicates l})
 }
+
+let rec all_elements
+  (#a:eqtype)
+  (l:count_list a)
+  (f:((a & count) -> bool))
+  : Tot bool (decreases l) =
+  match l with
+  | [] -> true
+  | hd::tl -> if f hd then all_elements tl f else false
+
 
 val spec_insert_element:
   bf:spec_bloom_storage_u8 ->
   e:element ->
   Tot spec_bloom_storage_u8
 let spec_insert_element bf e =
-  if FStar.Map.contains bf.map e then
-    let old_count = FStar.Map.sel bf.map e in
-    let new_map = FStar.Map.upd bf.map e (old_count + 1) in
-    if old_count = 0 then
-      { map = new_map; elements = e::bf.elements}
-    else
-      {bf with map = new_map }
+  if contains bf.elements e then
+    { bf with elements = incr_count bf.elements e }
   else
-    { map = FStar.Map.upd bf.map e 1; elements = e::bf.elements }
-
-let rec list_remove (#a:eqtype) (l:list a) (e:a) : Tot (list a) (decreases l)=
-  match l with
-  | [] -> l
-  | hd::tl ->
-    let new_tl = list_remove tl e in
-    if hd = e then new_tl else hd::new_tl
+    { bf with elements = (e,1)::bf.elements }
 
 val spec_remove_element:
   bf:spec_bloom_storage_u8 ->
   e:element ->
   Tot spec_bloom_storage_u8
 let spec_remove_element bf e =
-  if FStar.Map.contains bf.map e then
-    let old_count = FStar.Map.sel bf.map e in
-    if old_count = 0 then bf else
-      { map = FStar.Map.upd bf.map e (old_count - 1); elements = list_remove bf.elements e }
+  if contains bf.elements e  then
+    { bf with elements = decr_count bf.elements e }
   else
     bf
